chapter06/solutions/exercise01_solution.dfy
@@ -1,128 +1,92 @@
-include "../framework.s.dfy"
+//Your goal is to build a distributed lock server. This challenge differs from
+//LockServer in two ways. First, there is no central server that coordinates
+//the activity. Second, the hosts can communicate only via asynchronous
+//messages; a single state machine transition cannot simultaneously read or
+//update the state of two hosts.
+//
+//To guard against duplicate messages, the nodes associate a monotonically
+//increasing epoch number with the lock. Initially, node 0 holds the lock and
+//its epoch number is 1. A node that holds the lock can “grant” it to another
+//node by sending them a “Grant” message which has an epoch number that is
+//greater than the node’s epoch number. A node that receives such a message
+//will become the new holder and will set its epoch number to the message’s
+//epoch number.  
 
-//////////////////////////////////////////////////////////////////////////////
-// Protocol
+include "distributed_system.s.dfy"
 
-module Host {
-  import opened Base
-
-  datatype Message = Grant(dest:HostId, epoch:int)
-
-  datatype Constants = Constants(id:HostId)
-  datatype Variables = Variables(holdsLock:bool, epoch:int)
-
-  predicate DoGrant(k:Constants, s:Variables, s':Variables, a:NetAction<Message>, recipient:HostId) {
-    && s.holdsLock == true
-    && a.rcv.None?
-    && a.send == {Grant(recipient, s.epoch + 1)}
-    && s'.holdsLock == false
-    && s'.epoch == s.epoch
-  }
-
-  predicate DoAccept(k:Constants, s:Variables, s':Variables, a:NetAction<Message>) {
-    && a.rcv.Some?
-    && a.rcv.value.dest == k.id
-    && a.rcv.value.epoch > s.epoch
-    && a.send == {}
-    && s'.epoch == a.rcv.value.epoch
-    && s'.holdsLock == true
-  }
-
-  datatype Step = GrantStep(recipient:HostId) | AcceptStep()
-
-  predicate NextStep(k:Constants, s:Variables, s':Variables, a:NetAction<Message>, step:Step) {
-    match step {
-      case GrantStep(recipient) => DoGrant(k, s, s', a, recipient)
-      case AcceptStep() => DoAccept(k, s, s', a)
-    }
-  }
-
-  predicate Init(k:Constants, s:Variables, id:HostId) {
-    && k.id == id
-    && s.holdsLock == (id == 0)
-    && s.epoch == if id == 0 then 1 else 0
-  }
+predicate Safety(s:DistState) {
+  && WFState(s)
+  && forall i, j :: s.hosts[i].holdsLock && s.hosts[j].holdsLock ==> i == j
 }
 
-module DistributedLock refines DistributedSystem {
-  import Host
-
-  type M = Host.Message
-  type HConstants = Host.Constants
-  type HVariables = Host.Variables
-  type HStep(!new,==) = Host.Step
-
-  predicate HInit(k:HConstants, s:HVariables, id:HostId) {
-    Host.Init(k, s, id)
-  }
-
-  predicate HNextStep(k:HConstants, s:HVariables, s':HVariables, a:NetAction<M>, step:HStep) {
-    Host.NextStep(k, s, s', a, step)
-  }
+predicate InFlight(s:DistState, message:Message) {
+  && WFState(s)
+  && message in s.network.messageSet
+  && message.epoch > s.hosts[message.dest].epoch
 }
 
-//////////////////////////////////////////////////////////////////////////////
-// Proof
-// TODO separate the statement of the proof in a .s-ish way, per
-// sharded-hash-table.dfy
+predicate UniqueMessageInFlight(s:DistState) {
+  forall m1, m2 :: InFlight(s, m1) && InFlight(s, m2) ==> m1 == m2
+}
 
-module Proof {
-  import opened DistributedLock
+predicate InFlightPrecludesLockHeld(s:DistState) {
+  forall m :: InFlight(s, m) ==> (forall id :: !s.hosts[id].holdsLock)
+}
 
-  predicate Safety(k:Constants, s:Variables) {
-    && WFState(k, s)
-    && forall i, j :: s.hosts[i].holdsLock && s.hosts[j].holdsLock ==> i == j
-  }
+predicate InFlightHasFreshestEpoch(s:DistState) {
+  forall m :: InFlight(s, m) ==> (forall id :: s.hosts[id].epoch < m.epoch)
+}
 
-  predicate InFlight(k:Constants, s:Variables, message:M) {
-    && WFState(k, s)
-    && message in s.network.messageSet
-    && message.epoch > s.hosts[message.dest].epoch
-  }
+predicate LockHolderPrecludesInFlight(s:DistState)
+  requires WFState(s)
+{
+  forall id :: s.hosts[id].holdsLock ==> (forall m :: !InFlight(s, m))
+}
 
-  predicate KIsSane(k:Constants) {
-    forall id :: id in k.hosts && k.hosts[id].id == id
-  }
+predicate LockHolderHasFreshestEpoch(s:DistState)
+  requires WFState(s)
+{
+  forall id :: s.hosts[id].holdsLock ==>
+    (forall oid :: oid!=id ==> s.hosts[oid].epoch < s.hosts[id].epoch)
+}
 
-  predicate Inv(k:Constants, s:Variables) {
-    && KIsSane(k)
-    && Safety(k, s)
-    && (forall m1, m2 :: InFlight(k, s, m1) && InFlight(k, s, m2) ==> m1 == m2)
-    && (forall m :: InFlight(k, s, m) ==>
-      && (forall id :: !s.hosts[id].holdsLock)
-      && (forall id :: s.hosts[id].epoch < m.epoch))
-    && (forall id :: s.hosts[id].holdsLock ==>
-      && (forall m :: !InFlight(k, s, m))
-      && (forall oid :: oid!=id ==> s.hosts[oid].epoch < s.hosts[id].epoch))
-  }
+predicate Inv(s:DistState) {
+  && WFState(s)
 
-  lemma InvInit(k:Constants, s:Variables, s':Variables)
-    requires Init(k, s)
-    ensures Inv(k, s)
-  {
-  }
+  // There are never two messages in flight.
+  && UniqueMessageInFlight(s)
 
-  lemma InvNext(k:Constants, s:Variables, s':Variables)
-    requires Next(k, s, s')
-    requires Inv(k, s)
-    ensures Inv(k, s')
-  {
-    var id, a, step :| NextStep(k, s, s', id, a, step);
+  // If a message is flight, no client holds the lock, and
+  // the message has the freshest epoch number.
+  && InFlightPrecludesLockHeld(s)
+  && InFlightHasFreshestEpoch(s)
 
-    if step.AcceptStep? {
-      var message := a.rcv.value;
-      assert message.epoch > s.hosts[id].epoch;
-      assert message.epoch > s.hosts[message.dest].epoch;
-      assert forall i :: !s.hosts[i].holdsLock;
-      assert (forall id :: s'.hosts[id].holdsLock ==>
-        && (forall m :: !InFlight(k, s', m))
-        && (forall oid :: oid!=id ==> s'.hosts[oid].epoch < s'.hosts[id].epoch));
+  // If a clent holds the lock, no message is in flight, and
+  // the client has the freshest epoch number.
+  && LockHolderPrecludesInFlight(s)
+  && LockHolderHasFreshestEpoch(s)
+
+  && Safety(s)
+}
+
+lemma SafetyProof()
+  ensures forall s :: DistInit(s) ==> Inv(s)
+  ensures forall s, s' :: Inv(s) && DistNext(s, s') ==> Inv(s')
+  ensures forall s :: Inv(s) ==> Safety(s)
+{
+  forall s, s' | Inv(s) && DistNext(s, s') ensures Inv(s') {
+    var id, a :| NextStep(s, s', id, a);
+    if DoAccept(id, s.hosts[id], s'.hosts[id], a) {
+      assert UniqueMessageInFlight(s);  // observe
+      assert forall m | InFlight(s', m) :: InFlight(s, m);  // observe
+      forall m ensures !InFlight(s', m) {
+        assert InFlight(s, a.rcv.value);  // observe
+        assert !InFlight(s', a.rcv.value);  // observe
+      }
+      assert Inv(s'); // observe
+    } else {
+      var recipient :| DoGrant(s.hosts[id], s'.hosts[id], a, recipient); // observe
+      assert Inv(s'); // observe
     }
-  }
-
-  lemma InvImpliesSafety(k:Constants, s:Variables)
-    requires Inv(k, s)
-    ensures Safety(k, s)
-  {
   }
 }
