chapter06/exercises/protocol.i.dfy
@@ -1,0 +1,21 @@
+// Your protocol: message type, state machine
+
+include "network.s.dfy"
+
+// Define your Message datatype here.
+datatype Message = Message(/* FILL ME IN! */)
+
+// Define your Host protocol state machine here.
+datatype HostState = HostState(/* FILL ME IN! */)
+
+predicate HostInit(s:HostState, id:HostId) {
+  true
+}
+
+// The (trusted) DistributedSystem helpfully tells the host what its id is,
+// so the host can tell which messages are addressed to it. In a real system,
+// that id would be a constant part of the hosts' state; here we're trying
+// to keep the boilerplate to a minimum.
+predicate HostNext(id:HostId, s:HostState, s':HostState, a:NetAction<Message>) {
+  true
+}
