chapter06/solutions/distributed_system.s.dfy
@@ -1,0 +1,1 @@
+../exercises/distributed_system.s.dfy
