chapter06/solutions/network.s.dfy
@@ -1,0 +1,1 @@
+../exercises/network.s.dfy
