chapter06/solutions/protocol.i.dfy
@@ -1,0 +1,40 @@
+// Your protocol: message type, state machine
+
+include "network.s.dfy"
+
+// Define your Message datatype here.
+datatype Message = Grant(dest:HostId, epoch:nat)
+
+// Define your Host protocol state machine here.
+datatype HostState = HostState(holdsLock:bool, epoch:nat)
+
+predicate HostInit(s:HostState, id:HostId) {
+  && s.holdsLock == (id == 0)
+  && s.epoch == if id == 0 then 1 else 0
+}
+
+predicate DoGrant(s:HostState, s':HostState, a:NetAction<Message>, recipient:HostId) {
+  && s.holdsLock == true
+  && a.rcv.None?
+  && a.send == {Grant(recipient, s.epoch + 1)}
+  && s'.holdsLock == false
+  && s'.epoch == s.epoch
+}
+
+predicate DoAccept(id:HostId, s:HostState, s':HostState, a:NetAction<Message>) {
+  && a.rcv.Some?
+  && a.rcv.value.dest == id
+  && a.rcv.value.epoch > s.epoch
+  && a.send == {}
+  && s'.epoch == a.rcv.value.epoch
+  && s'.holdsLock == true
+}
+
+// The (trusted) DistributedSystem helpfully tells the host what its id is,
+// so the host can tell which messages are addressed to it. In a real system,
+// that id would be a constant part of the hosts' state; here we're trying
+// to keep the boilerplate to a minimum.
+predicate HostNext(id:HostId, s:HostState, s':HostState, a:NetAction<Message>) {
+  || (exists recipient :: DoGrant(s, s', a, recipient) )
+  || DoAccept(id, s, s', a)
+}
